theories/zoo_std/inf_array__code.v
@@ -49,21 +49,23 @@ Definition inf_array_get : val :=
            "t".{default}
          )).
 
-Definition inf_array_set : val :=
-  fun: "t" "i" "v" =>
+Definition inf_array_update : val :=
+  fun: "t" "i" "fn" =>
     mutex_protect "t".{mutex}
       (fun: <> =>
          inf_array_reserve "t" ("i" + #1) ;;
-         array_unsafe_set "t".{data} "i" "v").
+         let: "v" := array_unsafe_get "t".{data} "i" in
+         array_unsafe_set "t".{data} "i" ("fn" "v") ;;
+         "v").
 
 Definition inf_array_xchg : val :=
   fun: "t" "i" "v" =>
-    mutex_protect "t".{mutex}
-      (fun: <> =>
-         inf_array_reserve "t" ("i" + #1) ;;
-         let: "v'" := array_unsafe_get "t".{data} "i" in
-         array_unsafe_set "t".{data} "i" "v" ;;
-         "v'").
+    inf_array_update "t" "i" (fun: <> => "v").
+
+Definition inf_array_set : val :=
+  fun: "t" "i" "v" =>
+    inf_array_xchg "t" "i" "v" ;;
+    ().
 
 Definition inf_array_cas : val :=
   fun: "t" "i" "v1" "v2" =>
@@ -79,9 +81,4 @@ Definition inf_array_cas : val :=
 
 Definition inf_array_faa : val :=
   fun: "t" "i" "incr" =>
-    mutex_protect "t".{mutex}
-      (fun: <> =>
-         inf_array_reserve "t" ("i" + #1) ;;
-         let: "n" := array_unsafe_get "t".{data} "i" in
-         array_unsafe_set "t".{data} "i" ("n" + "incr") ;;
-         "n").
+    inf_array_update "t" "i" (fun: "n" => "n" + "incr").
